A few more refactor and progress case

Bigstep.v
@@ -21,21 +21,21 @@ Definition get_this_var_mapping (vm : var_mapping) : option Loc :=
 
 (* Get the runtime mutability type of a Loc *)
 Definition r_muttype (h: heap) (ι: Loc) : option q_r :=
-  match getObj h ι with
+  match runtime_getObj h ι with
   | None => None
   | Some o => Some (rqtype (rt_type o))
   end.
 
 (* Get the runtime class name of a Loc *)
 Definition r_basetype (h: heap) (ι: Loc) : option class_name :=
-  match getObj h ι with
+  match runtime_getObj h ι with
   | None => None
   | Some o => Some (rctype (rt_type o))
   end.
 
 (* Get the runtime type of a Loc *)
 Definition r_type (h: heap) (ι: Loc) : option runtime_type :=
-  match getObj h ι with
+  match runtime_getObj h ι with
   | None => None
   | Some o => Some (rt_type o)
   end.
@@ -94,7 +94,7 @@ Definition can_assign (CT: class_table) (rΓ: r_env) (h: heap) (ι: Loc) (f: var
   end.
 
 Definition update_field (h: heap) (ι: Loc) (f: var) (v: value) : heap :=
-  match getObj h ι with
+  match runtime_getObj h ι with
   | None => h
   | Some o =>
       let new_fields := update f v o.(fields_map) in
@@ -116,20 +116,27 @@ Definition wf_rtypeuse (CT: class_table) (q: q_r) (c: class_name) : Prop :=
 
 (* Wellformed Runtime Object: an object is well-formed if itself and its fields' type are well formed *)
 Definition wf_obj (CT: class_table) (h: heap) (ι: Loc) : Prop :=
-  match getObj h ι with
+  match runtime_getObj h ι with
   | None => False
   | Some o =>
+      (* The runtime type of the object is well-formed *)
       wf_rtypeuse CT (rt_type o).(rqtype) (rt_type o).(rctype) /\
+      (* The runtime type of the object's fields are well-formed *)
+      (* TODO: think about this, maybe the second case is not needed. Field type and runtime value type*)
       Forall (fun v =>
         match v with
         | Null_a => True
         | Iot loc =>
-            match getObj h loc with
+            match runtime_getObj h loc with
             | None => False
             | Some o' => wf_rtypeuse CT (rt_type o').(rqtype) (rt_type o').(rctype)
             end
-        end) (fields_map o)
+        end) (fields_map o) /\
+      (* The number of fields are the same at runtime and static type *)
+      List.length (fields_map o) = List.length (collect_fields CT (rt_type o).(rctype))
   end.
+
+(* TODO: here I need extra lemma that sub class have equal or more fields *)
 
 (* Wellformed Runtime environment: a rΓ is well formed if for all variable in its domain, it maps to null_a or a value in the domin of heap *)
 Definition wf_renv (CT: class_table) (rΓ: r_env) (h: heap) : Prop :=
@@ -137,11 +144,27 @@ Definition wf_renv (CT: class_table) (rΓ: r_env) (h: heap) : Prop :=
     match value with
     | Null_a => True
     | Iot loc =>
-        match getObj h loc with
+        match runtime_getObj h loc with
         | None => False
         | Some _ => True
         end
     end) rΓ.(vars).
+
+(* Lemma object_not_he_than_renv : forall CT rΓ h,
+    wf_renv CT rΓ h ->
+    runtime_getObj_.
+Proof.
+  intros CT rΓ h Hwf.
+  unfold wf_renv in Hwf.
+  remember (List.length h) as n.
+  induction n as [|n' IH].
+  - lia.
+  - replace (S n') with (List.length h) by (symmetry; exact Heqn).
+    remember (List.length h) as n.
+    remember (List.length rΓ.(vars)) as m.
+
+    lia.
+Qed. *)
 
 (* Wellformed Runtime Heap: a heap is well-formed if all objects in it are well-formed *)
 Definition wf_heap (CT: class_table) (h: heap) : Prop :=
@@ -178,7 +201,7 @@ Definition wf_r_config (CT: class_table) (sΓ: s_env) (rΓ: r_env) (h: heap)  : 
   forall i, i < List.length sΓ ->
   forall sqt,
     nth_error sΓ i = Some sqt ->
-    match getVal rΓ.(vars) i with
+    match runtime_getVal rΓ i with
     | Some (Iot loc) => wf_r_typable CT rΓ h loc sqt
     | Some Null_a => True
     | None => False
@@ -188,25 +211,28 @@ Lemma not_in_both_env: forall CT sΓ rΓ h,
     List.length sΓ = List.length rΓ.(vars)->
     forall i, i < List.length sΓ ->
     forall sqt, nth_error sΓ i = Some sqt ->
-    match getVal rΓ.(vars) i with
+    match runtime_getVal rΓ i with
     | Some (Iot loc) => wf_r_typable CT rΓ h loc sqt
     | Some Null_a => True
     | None => False
-    end -> (forall x, x >= List.length sΓ -> static_lookup sΓ x = None -> getVal (vars rΓ) x = None).
+    end -> (forall x, x >= List.length sΓ -> (static_getType sΓ x = None <-> runtime_getVal rΓ x = None)).
 Proof.
 intros.
-unfold static_lookup in H1.
+unfold static_getType in H1.
 destruct (lt_dec x (List.length sΓ)). 
   - (* x < dom sΓ *)
-    unfold getVal.
+    unfold runtime_getVal.
     rewrite nth_error_None.
     rewrite <- H.
     lia.
   - (* x >= dom sΓ *)
-    unfold getVal.
+    unfold runtime_getVal.
     rewrite nth_error_None.
     rewrite <- H.
-    lia.
+    split.
+    + lia.
+    + unfold static_getType.
+      apply nth_error_None.
 Qed.
 
 Global Hint Resolve not_in_both_env: rch.
@@ -222,14 +248,15 @@ Inductive eval_expr : r_env -> heap -> expr -> value -> r_env -> heap -> Prop :=
 
   (* evaluate value expression *)
   | EBS_Val : forall rΓ h x v,
-      getVal rΓ.(vars) x = Some v ->
+      runtime_getVal rΓ x = Some v ->
       eval_expr rΓ h (EVar x) v rΓ h
 
   (* evaluate field access expression *)  
-  | EBS_Field : forall rΓ h x f (v:value) v o,
-      getObj h x = Some o ->
-      getVal o.(fields_map) f = Some v ->
-      eval_expr rΓ h (EField x f) v rΓ h
+  | EBS_Field : forall rΓ h x f v o v1,
+      runtime_getVal rΓ x = Some (Iot v) ->
+      runtime_getObj h v = Some o ->
+      getVal o.(fields_map) f = Some v1 ->
+      eval_expr rΓ h (EField x f) v1 rΓ h
   .
 Notation "'(' rΓ ',' h ')' '⟦'  e  '⟧'   '-->'  '(' v ',' rΓ' ',' h' ')'" := (eval_expr rΓ h e v rΓ' h') (at level 80).
 
@@ -241,7 +268,7 @@ Inductive eval_stmt : r_env -> heap -> stmt -> r_env -> heap -> Prop :=
 
   (* evaluate local variable declaration statement *)
   | SBS_Local : forall rΓ h T x,
-      getVal rΓ.(vars) x = None ->
+      runtime_getVal rΓ x = None ->
       eval_stmt rΓ h (SLocal T x)
       (* (rΓ <|vars := update (List.length rΓ.(vars) + 1) Null_a rΓ.(vars)|> <|init_state := rΓ.(init_state)|>) *)
       (rΓ <|vars := update (List.length rΓ.(vars) + 1) Null_a rΓ.(vars)|> )
@@ -249,7 +276,7 @@ Inductive eval_stmt : r_env -> heap -> stmt -> r_env -> heap -> Prop :=
 
   (* evaluate variable assignment statement *)
   | SBS_Assign : forall rΓ h x e v1 v2,
-      getVal rΓ.(vars) x = Some v1 ->
+      runtime_getVal rΓ x = Some v1 ->
       eval_expr rΓ h e v2 rΓ h ->
       eval_stmt rΓ h (SVarAss x e)
       (* (rΓ <|vars := update x v2 rΓ.(vars)|> <|init_state := rΓ.(init_state)|>) *)
@@ -257,18 +284,18 @@ Inductive eval_stmt : r_env -> heap -> stmt -> r_env -> heap -> Prop :=
       h
 
   (* evaluate field write statement *)
-  | SBS_FldWrite: forall CT rΓ h x f y v1 lx v2 h',
-      getVal rΓ.(vars) x = Some v1 ->
-      v1 = Iot lx ->
-      getVal rΓ.(vars) y = Some v2 ->
+  | SBS_FldWrite: forall CT rΓ h x f y lx o vf v2 h',
+      runtime_getVal rΓ x = Some (Iot lx) ->
+      runtime_getObj h lx = Some o ->
+      getVal o.(fields_map) f = Some vf ->
+      runtime_getVal rΓ y = Some v2 ->
       can_assign CT rΓ h lx f = true ->
       h' = update_field h lx f v2 ->
       eval_stmt rΓ h (SFldWrite x f y) rΓ h'
 
   (* evaluate object creation statement *)
-  | SBS_New: forall rΓ h x q_c c ys vals v l1 qthisr qthis qadapted o rΓ' h',
-      getVal rΓ.(vars) 0 = Some v ->
-      v = Iot l1 ->
+  | SBS_New: forall rΓ h x q_c c ys vals l1 qthisr qthis qadapted o rΓ' h',
+      runtime_getVal rΓ 0 = Some (Iot l1) ->
       runtime_lookup_list rΓ ys = Some vals ->
       r_muttype h l1 = Some qthisr ->
       qthis = q_r_proj qthisr ->
@@ -280,7 +307,7 @@ Inductive eval_stmt : r_env -> heap -> stmt -> r_env -> heap -> Prop :=
 
   (* evaluate method call statement *)
   | SBS_Call: forall CT rΓ h x y m zs vals ly cy mbody mstmt mret retval h' rΓ' rΓ'' rΓ''',
-    getVal rΓ.(vars) y = Some (Iot ly) ->
+    runtime_getVal rΓ y = Some (Iot ly) ->
     r_basetype h ly = Some cy ->
     method_body_lookup CT cy m = Some mbody ->
     mstmt = mbody.(mbody_expr) ->
@@ -289,7 +316,7 @@ Inductive eval_stmt : r_env -> heap -> stmt -> r_env -> heap -> Prop :=
     (* rΓ' = mkr_env (Iot ly :: vals) rΓ.(init_state) -> *)
     rΓ' = mkr_env (Iot ly :: vals) ->
     eval_stmt rΓ' h mstmt rΓ'' h' ->
-    getVal rΓ''.(vars) mret = Some retval ->
+    runtime_getVal rΓ'' mret = Some retval ->
     rΓ''' = rΓ <| vars := update x retval rΓ.(vars) |> ->
     eval_stmt rΓ h (SCall x m y zs) rΓ''' h'
 
